
$$
\begin{align}
c'=&0 \\
(cu)'=&cu' \\
(u\pm v)'=&u'\pm v' \\
(uv)'=&u'v+uv' \\
\prod_{i=1}^{n} u_{i}=&\sum_{i=1}^{n}u_{1}\cdots u_{i}'\cdots u_{n} \\
\left( \frac{u}{v} \right)'=&\frac{{u'v-uv'}}{v^2} \\
[u(v(w(x)))]'=&\frac{du}{dv} \frac{dv}{dw} \frac{dw}{dx} \\
(u^\alpha)'=&\alpha u^{\alpha-1}u' \\
y=f(x),x=\varphi(y)\iff& f'(x)=\frac{1}{\varphi'(y)} \\
F(x,y)=0\iff& F_{x}+F_{y}y'=0 \\
x=x(t),y=y(t)\iff& y'=\frac{dy}{dx}=\frac{y'(t)}{x'(t)} \\
\rho=\rho(\varphi)\iff& x=\rho(\varphi)\cos \varphi,y=\rho(\varphi)\sin \varphi, \\
&y'=\frac{{\dot{\rho}\sin \varphi+\rho \cos \varphi}}{\dot{\rho}\cos \varphi-\rho \sin \varphi}\left( \dot{\rho}=\frac{d\rho}{d\varphi} \right) \\ \\
(uv)^{(n)}=&\sum_{m=1}^{n}C_{n}^{m}u^{(m)}v^{(n-m)} \\
x=x(t),y=y(t)\iff& \frac{d^2y}{dx^2}=\frac{{\dot{x}\ddot{y}-\dot{y}\ddot{x}}}{\dot{x}^3},  \\
&\frac{d^3y}{dx^3}=\frac{{\dot{x}^2\dddot{y}-3\dot{x}\ddot{x}\ddot{y}+3\dot{y}\ddot{x}^2-\dot{x}\dot{y}\dddot{x}}}{\dot{x}^5}\\&\cdots  \\
&\left( \dot{y}=\frac{dy}{dt},\dot{x}=\frac{dx}{dt} \cdots\right)
\end{align}
$$
